# **Inverse Function**

### **Definition**

* An inverse function reverses the action of a given function.
* Let $ f : A \to B $ be a function.
* If there exists a function $ f^{-1} : B \to A $ such that
  $$
  f^{-1}(f(x)) = x \quad \text{for all } x \in A
  $$
  and
  $$
  f(f^{-1}(y)) = y \quad \text{for all } y \in B,
  $$
  then $ f^{-1} $ is called the inverse of ( f ).
* An inverse exists **only if the function is bijective**.

---

### **Examples**

* If $ f(x) = x + 3 $, then
  $ f^{-1}(x) = x - 3 $.
* If $ f(x) = 2x $, then
  $ f^{-1}(x) = \frac{x}{2} $.
* Applying a function and its inverse gives the original value.

---

### **Rules for Inverse Function**

* The function must be **one-to-one and onto**.
* The **domain of ( f )** becomes the **codomain of $ f^{-1} $**.
* The **codomain of ( f )** becomes the **domain of $ f^{-1} $**.
* To find an inverse:

  * Replace ( f(x) ) with ( y ).
  * Interchange ( x ) and ( y ).
  * Solve for ( y ).
  * $ f^{-1} $ does **not** mean reciprocal of ( f ).

---

### **Properties of Inverse Function**

* $ f \circ f^{-1} = I $ (identity function).
* $ f^{-1} \circ f = I $.
* $ (f^{-1})^{-1} = f $.
* If ( f ) and ( g ) are bijections, then
  $$
  (g \circ f)^{-1} = f^{-1} \circ g^{-1}
  $$.

---

